Hoare remain Repeat, Assert and Assume

plf/Hoare.v
@@ -382,7 +382,9 @@ Theorem hoare_post_true : forall (P Q : Assertion) c,
   (forall st, Q st) ->
   {{P}} c {{Q}}.
 Proof.
-  (* FILL IN HERE *) Admitted.
+  unfold valid_hoare_triple. intros P c Q H st st' H1 Pre.
+  auto.
+Qed.
 (** [] *)
 
 (** **** Exercise: 1 star, standard (hoare_pre_false) *)
@@ -394,7 +396,9 @@ Theorem hoare_pre_false : forall (P Q : Assertion) c,
   (forall st, ~ (P st)) ->
   {{P}} c {{Q}}.
 Proof.
-  (* FILL IN HERE *) Admitted.
+  unfold valid_hoare_triple. intros P c Q H st st' H1 Pre.
+  apply H in Pre. contradiction.
+Qed.
 (** [] *)
 
 (* ################################################################# *)
@@ -449,6 +453,9 @@ Proof.
   intros P Q R c1 c2 H1 H2 st st' H12 Pre.
   inversion H12; subst.
   eauto.
+  (* apply (H2 st st'0 H3) in Pre.
+  apply (H1 st'0 st' H6) in Pre.
+  apply Pre. *)
 Qed.
 
 (** Note that, in the formal rule [hoare_seq], the premises are
@@ -693,7 +700,8 @@ Example hoare_asgn_examples1 :
       X := 2 * X
     {{ X <= 10 }}.
 Proof.
-  (* FILL IN HERE *) Admitted.
+  exists ({{(X <= 10) [X |-> 2 * X]}}).
+  apply hoare_asgn. Qed.
 (** [] *)
 
 (** **** Exercise: 2 stars, standard, optional (hoare_asgn_examples2) *)
@@ -702,7 +710,9 @@ Example hoare_asgn_examples2 :
     {{ P }}
       X := 3
     {{ 0 <=  X /\ X <= 5 }}.
-Proof. (* FILL IN HERE *) Admitted.
+Proof. 
+  exists ({{(0 <= X /\ X <= 5) [X |-> 3]}}).
+  apply hoare_asgn. Qed.
 (** [] *)
 
 (** **** Exercise: 2 stars, standard, especially useful (hoare_asgn_wrong) *)
@@ -724,10 +734,18 @@ Proof. (* FILL IN HERE *) Admitted.
 Theorem hoare_asgn_wrong : exists a:aexp,
   ~ {{ True }} X := a {{ X = a }}.
 Proof.
-  (* FILL IN HERE *) Admitted.
-(* FILL IN HERE
-
-    [] *)
+  exists (<{X+1}>). unfold valid_hoare_triple, not.
+  intros. 
+  remember ((X !-> 1):state) as st.
+  remember ((X !-> 2; X !-> 1):state) as st'.
+  assert (goal: st =[ X := X + 1 ]=> st').
+  { subst. apply E_Asgn. simpl. reflexivity. }
+  remember (H st st' goal I) as contra. 
+  subst st'. unfold t_update in contra. simpl in contra.  
+  discriminate.
+Qed.
+ 
+(* [] *)
 
 (** **** Exercise: 3 stars, advanced (hoare_asgn_fwd)
 
@@ -755,7 +773,14 @@ Theorem hoare_asgn_fwd :
   {{ $(fun st => (P (X !-> m ; st)
              /\ st X = aeval (X !-> m ; st) a))  }}.
 Proof.
-  (* FILL IN HERE *) Admitted.
+  intros m a P st st' Hst Pre. inversion Hst; subst; simpl in *.
+  destruct Pre as [Hp Hm].
+  assert (goal: (X !-> m; X !-> aeval st a; st) = st).
+  { rewrite t_update_shadow. rewrite <- Hm. rewrite t_update_same. auto. }
+  rewrite goal. split. 
+  - assumption.
+  - reflexivity.
+Qed. 
 (** [] *)
 
 (** **** Exercise: 2 stars, advanced, optional (hoare_asgn_fwd_exists)
@@ -778,7 +803,15 @@ Theorem hoare_asgn_fwd_exists :
   {{ $(fun st => exists m, P (X !-> m ; st) /\
                 st X = aeval (X !-> m ; st) a) }}.
 Proof.
-  (* FILL IN HERE *) Admitted.
+  intros a P st st' Hst Pre. inversion Hst; subst; simpl in *.
+  exists (st X).
+  assert (goal: (X !-> st X; X !-> aeval st a; st) = st).
+  { rewrite t_update_shadow. rewrite t_update_same. auto. }
+  split.
+  - rewrite goal. auto. 
+  - rewrite goal. reflexivity.
+Qed. 
+
 (** [] *)
 
 (* ================================================================= *)
@@ -1109,14 +1142,20 @@ Example assertion_sub_ex1' :
     X := 2 * X
   {{ X <= 10 }}.
 Proof.
-  (* FILL IN HERE *) Admitted.
+  eapply hoare_consequence_pre.
+  - apply hoare_asgn.
+  - assertion_auto.
+Qed.
 
 Example assertion_sub_ex2' :
   {{ 0 <= 3 /\ 3 <= 5 }}
     X := 3
   {{ 0 <= X /\ X <= 5 }}.
 Proof.
-  (* FILL IN HERE *) Admitted.
+  eapply hoare_consequence_pre.
+  - apply hoare_asgn.
+  - assertion_auto.
+Qed.
 
 (** [] *)
 
@@ -1180,7 +1219,13 @@ Example hoare_asgn_example4 :
   {{ X = 1 /\ Y = 2 }}.
 Proof.
   eapply hoare_seq with (Q := {{ X = 1 }}).
-  (* FILL IN HERE *) Admitted.
+  - eapply hoare_consequence_pre.
+    + apply hoare_asgn.
+    + assertion_auto.
+  - eapply hoare_consequence_pre.
+    + apply hoare_asgn.
+    + assertion_auto.
+Qed.
 (** [] *)
 
 (** **** Exercise: 3 stars, standard (swap_exercise)
@@ -1201,15 +1246,29 @@ Proof.
          and work back to the beginning of your program.
        - Remember that [eapply] is your friend.)  *)
 
-Definition swap_program : com
-  (* REPLACE THIS LINE WITH ":= _your_definition_ ." *). Admitted.
+(* solving the problem with only one assignment *)
+Ltac asign_auto :=
+  eapply hoare_consequence_pre;
+  try (apply hoare_asgn); 
+  try (assertion_auto).
+
+Definition swap_program : com :=
+  <{ Z := X; 
+     X := Y; 
+     Y := Z }>.
 
 Theorem swap_exercise :
   {{X <= Y}}
     swap_program
   {{Y <= X}}.
 Proof.
-  (* FILL IN HERE *) Admitted.
+  unfold swap_program.
+  eapply hoare_seq with (Q := {{Z <= Y}}).
+  - eapply hoare_seq with (Q := {{Z <= X}}).
+    + asign_auto.
+    + asign_auto.
+  - asign_auto.
+Qed.
 (** [] *)
 
 (** **** Exercise: 4 stars, advanced (invalid_triple)
@@ -1250,7 +1309,16 @@ Theorem invalid_triple : ~ forall (a : aexp) (n : nat),
 Proof.
   unfold valid_hoare_triple.
   intros H.
-  (* FILL IN HERE *) Admitted.
+  specialize H with (a := <{ X + 1 }>) (n := 1) 
+    (st := (X !-> 0)) (st' := (Y !-> 4; X !-> 3; X !-> 0)).
+  simpl in *.
+  assert (Hpre: (X !-> 0) =[ X := 3; Y := X + 1 ]=> (Y !-> 4; X !-> 3; X !-> 0)).
+  { eapply E_Seq.
+    - eapply E_Asgn. reflexivity.
+    - eapply E_Asgn. reflexivity. }
+  remember (H Hpre (eq_refl 1)) as contra.
+  unfold t_update in contra. simpl in *. discriminate.
+Qed.
 (** [] *)
 
 (* ================================================================= *)
@@ -1430,6 +1498,10 @@ Ltac assertion_auto'' :=
   try rewrite -> leb_le in *;  (* for inequalities *)
   auto; try lia.
 
+Ltac unfold_assertion := 
+  unfold "->>", assertion_sub, t_update, bassertion;
+  intros; simpl in *.
+
 (** **** Exercise: 2 stars, standard (if_minus_plus)
 
     Prove the theorem below using [hoare_if].  Do not use [unfold
@@ -1444,7 +1516,14 @@ Theorem if_minus_plus :
     end
   {{Y = X + Z}}.
 Proof.
-  (* FILL IN HERE *) Admitted.
+  apply hoare_if.
+  - eapply hoare_consequence_pre.
+    + apply hoare_asgn.
+    + assertion_auto''.
+  - eapply hoare_consequence_pre.
+    + apply hoare_asgn.
+    + assertion_auto''.
+Qed.
 (** [] *)
 
 (* ----------------------------------------------------------------- *)
@@ -1529,7 +1608,13 @@ Inductive ceval : com -> state -> state -> Prop :=
       st  =[ c ]=> st' ->
       st' =[ while b do c end ]=> st'' ->
       st  =[ while b do c end ]=> st''
-(* FILL IN HERE *)
+  | E_If1True : forall st st' b c,
+      beval st b = true ->
+      st =[ c ]=> st' ->
+      st =[ if1 b then c end ]=> st'
+  | E_If1False : forall st b c,
+      beval st b = false ->
+      st =[ if1 b then c end ]=> st
 
 where "st '=[' c ']=>' st'" := (ceval c st st').
 
@@ -1540,11 +1625,11 @@ Hint Constructors ceval : core.
 
 Example if1true_test :
   empty_st =[ if1 X = 0 then X := 1 end ]=> (X !-> 1).
-Proof. (* FILL IN HERE *) Admitted.
+Proof. eauto. Qed.
 
 Example if1false_test :
   (X !-> 2) =[ if1 X = 0 then X := 1 end ]=> (X !-> 2).
-Proof. (* FILL IN HERE *) Admitted.
+Proof. eauto. Qed.
 
 (** [] *)
 
@@ -1581,7 +1666,18 @@ Notation "{{ P }} c {{ Q }}" :=
     be in the assertion scope.  For example, if you want [e] to be
     parsed as an assertion, write it as [(e)%assertion]. *)
 
-(* FILL IN HERE *)
+Theorem hoare_if1 : forall P Q (b:bexp) c,
+  {{P /\ b}} c {{Q}} ->
+  {{P /\ ~ b}} ->> Q ->
+  {{P}} if1 b then c end {{Q}}.
+Proof.
+  intros P Q b c HTure HFalse st st' HE HP.
+  inversion HE; subst.
+  - eapply HTure; eauto.
+  - eapply HFalse.
+    split; try (unfold not); assertion_auto''; rewrite H3 in H; discriminate. 
+Qed.
+
 
 (** For full credit, prove formally ([hoare_if1_good]) that your rule is
     precise enough to show the following Hoare triple is valid:
@@ -1592,6 +1688,7 @@ Notation "{{ P }} c {{ Q }}" :=
     end
   {{ X = Z }}
 *)
+
 (* Do not modify the following line: *)
 Definition manual_grade_for_hoare_if1 : option (nat*string) := None.
 (** [] *)
@@ -1635,7 +1732,17 @@ Lemma hoare_if1_good :
       X := X + Y
     end
   {{ X = Z }}.
-Proof. (* FILL IN HERE *) Admitted.
+Proof. 
+  apply hoare_if1.
+  - eapply hoare_consequence_pre.
+    + apply hoare_asgn.
+    + assertion_auto''.
+  - unfold_assertion.
+    destruct H as [Heq Hneq].
+    apply eq_true_negb_classical in Hneq. 
+    rewrite eqb_eq in Hneq.
+    rewrite Hneq in Heq. lia.
+Qed.
 (** [] *)
 
 End If1.
@@ -1705,6 +1812,12 @@ Proof.
   remember <{while b do c end}> as original_command eqn:Horig.
   induction Heval;
     try (inversion Horig; subst; clear Horig);
+    (* - eauto.
+    - apply IHHeval2.
+      + reflexivity.
+      + eapply Hhoare.
+        * apply Heval1.
+        * auto. *)
     eauto.
 Qed.
 
@@ -2061,13 +2174,15 @@ Proof. eauto. Qed.
 (** Complete the Hoare rule for [HAVOC] commands below by defining
     [havoc_pre], and prove that the resulting rule is correct. *)
 
-Definition havoc_pre (X : string) (Q : Assertion) (st : total_map nat) : Prop
-  (* REPLACE THIS LINE WITH ":= _your_definition_ ." *). Admitted.
+Definition havoc_pre (X : string) (Q : Assertion) (st : total_map nat) : Prop :=
+  forall n, Q (X !-> n ; st).
 
 Theorem hoare_havoc : forall (Q : Assertion) (X : string),
   {{ $(havoc_pre X Q) }} havoc X {{ Q }}.
 Proof.
-  (* FILL IN HERE *) Admitted.
+  intros Q X. unfold havoc_pre, valid_hoare_triple.
+  intros. inversion H; subst. apply H0.
+Qed.
 (** [] *)
 
 (** **** Exercise: 3 stars, advanced (havoc_post)
@@ -2085,8 +2200,12 @@ Theorem havoc_post : forall (P : Assertion) (X : string),
 Proof.
   intros P X. eapply hoare_consequence_pre.
   - apply hoare_havoc.
-  - (* FILL IN HERE *) Admitted.
-
+  - unfold "->>", havoc_pre. intros. 
+    exists (st X). unfold assertion_sub. simpl. 
+    assert (goal : (X !-> st X; X !-> n; st) = st).
+    { rewrite t_update_shadow, t_update_same. reflexivity. }
+    rewrite goal. apply H.
+Qed.
 (** [] *)
 
 End Himp.
